wip: linearization

src/spec/Flutterbye.Linearization.fst
@@ -23,82 +23,72 @@ open Flutterbye.Entropy
 
 type transaction_t 'a = 'a -> 'a
 
-type xnid_t (#a_t:Type) (s_xn:seq (transaction_t a_t)) =
-   | XnId: as_nat:nat{as_nat < length s_xn} -> xnid_t s_xn
+type xnid_t (#a_t:Type) (todo:seq (transaction_t a_t)) =
+   | XnId: as_nat:nat{as_nat < length todo} -> xnid_t todo
 
-type pending_t (#a_t:Type) (s_xn:seq (transaction_t a_t)) =
-   | Pending: id:xnid_t s_xn -> s:a_t -> pending_t s_xn
+type pending_t (#a_t:Type) (todo:seq (transaction_t a_t)) =
+   | Pending: id:xnid_t todo -> s:a_t -> pending_t todo
 
-type step_t (#a_t:Type) (s_xn:seq (transaction_t a_t)) =
-   | Next: id:xnid_t s_xn -> step_t s_xn
-   | Studder: id:xnid_t s_xn -> step_t s_xn
+type step_t (#a_t:Type) (todo:seq (transaction_t a_t)) =
+   | Next: id:xnid_t todo -> step_t todo
+   | Studder: id:xnid_t todo -> step_t todo
 
-val linearize_loop:
-   s_xn:seq (transaction_t 'a)
+type next_loop_p:
+   (#a_t:Type)
+   (xns:seq (transaction_t a_t))
+   (a:a_t)
+   (pending:seq (pending_t xns))
+   (steps':seq (step_t xns))
+=
+   length xns > 0
+   /\ (exists (x:nat{x < length pending}).
+         Pending.s (index pending x) = a)
+   /\ (exists (x:nat{x < length steps'}).
+         is_Next step (index steps' x)
+
+val next_loop:
+   xns:seq (transaction_t 'a)
    -> a:'a
-   -> p:seq (pending_t s_xn)
-   -> l:seq (step_t s_xn)
-   -> Tot (l':seq (step_t 'a))
+   -> pending:seq (pending_t xns)
+   -> steps:seq (step_t xns)
+   -> Tot (steps':seq (step_t xns){next_loop_p xns a pending steps'})
       decreases (length p)
-let rec linearize_loop s_xn a p l =
+let rec next_loop xns a pending steps =
    if length p = 0 then
-      l
+      steps
    else
       let i = 0 in
-      let xn_p = index p i in
-      let xnid = Pending.id xn_p in
-      let allow = (Pending.s xn_p = a) in
+      let pending = index p i in
+      let xnid = Pending.id pending in
+      let allow = (Pending.s pending = a) in
       if allow
-         // step 
+         append (create (Step xnid) 1) in
       else
-         // todo: i'll bet this needs to be two loops!
-         let l' = append (create (Studder xnid) 1) in
+         let steps' = append (create (Studder xnid) 1) in
          let retry = Pending xnid a in
          let p' = append (remove p i) (create retry 1) in
-         linearize_loop s_xn a p' l'
+         linearize_loop xns a p' steps'
 
-
-      let s' = 
-         if allow then
-            let f = index s_xn (XnId.as_nat xnid) in
-            f s
-         else
-            s
-      in
-      let p' = 
-         if allow then
-            remove p i
-         else
-            p
-      in
-      let l' = 
-         if allow then
-            append (create (Step xnid) 1)
-         else
-            append (create (Studder xnid) 1)
-      in
-
-   
-type linearized_p (#a_t:Type) (#b_t:Type) (s_xn:seq (transaction_t a_t)) (s_0:a_t) (l:seq (step_t s_xn)) =
-   length s_xn = 0
+(*type linearized_p (#a_t:Type) (#b_t:Type) (todo:seq (transaction_t a_t)) (s_0:a_t) (l:seq (step_t todo)) =
+   length todo = 0
    \/ // every transaction has a corresponding `Step` operation in
       // the linearization sequence.
-      forall (x:xnid_t s_xn).
+      forall (x:xnid_t todo).
          (exists (y:nat{y < length l}).
             let op = index l y in
             is_Step op && Step.id op = x)
 
 val linearize:
-   s_xn:seq (transaction_t 'a)
+   todo:seq (transaction_t 'a)
    -> s_0:'a
    -> e:entropy_t 'b
-   -> Tot (l:seq (step_t 'a)){linearized_p s_xn s_0 l})
-let linearize s_xn s_0 =
+   -> Tot (l:seq (step_t 'a)){linearized_p todo s_0 l})
+let linearize todo s_0 =
    let p = 
       map
          (fun i x ->
             Pending i s_0)
-         s_xn
+         todo
    in
-   linearize_loop s_xn p createEmpty*)
-
+   linearize_loop todo p createEmpty*)
+*)
